cleanup

src/Experiments/Loops.v
@@ -16,47 +16,60 @@ Module Import core.
   Section Loops.
     Context {A B : Type} (body : A -> A + B).
 
+    (* the fuel parameter is only present to allow defining a loop
+    without proving its termination. The loop body does not have
+    access to the amount of remaining fuel, and thus increasing fuel
+    beyond termination cannot change the behavior. fuel counts full
+    loops -- the one that exacutes "break" is not included *)
+
     Fixpoint loop (fuel : nat) (s : A) {struct fuel} : A + B :=
-      match fuel with
-      | O => inl s
-      | S fuel' =>
-        let s := body s in
-        match s with
-        | inl a => loop fuel' a
-        | inr b => inr b
-        end
+      let s := body s in
+      match s with
+      | inl a =>
+        match fuel with
+        | O => inl a
+        | S fuel' => loop fuel' a
+        end 
+      | inr b => inr b
       end.
 
     Context (body_cps : A ~> A + B).
 
     Fixpoint loop_cps (fuel : nat) (s : A) {struct fuel} :~> A + B :=
-      match fuel with
-      | O => return (inl s)
-                  | S fuel' =>
-                    s <- body_cps s;
-                      match s with
-                      | inl a => loop_cps fuel' a
-                      | inr b => return (inr b)
-                      end
-      end.
+      s <- body_cps s;
+        match s with
+        | inl a => 
+          match fuel with
+          | O => return (inl a)
+          | S fuel' => loop_cps fuel' a
+          end
+        | inr b => return (inr b)
+        end.
 
     Context (body_cps_ok : forall s {R} f, body_cps s R f = f (body s)).
     Lemma loop_cps_ok n s {R} f : loop_cps n s R f = f (loop n s).
     Proof.
-      revert f; revert R; revert s; induction n; [reflexivity|]; cbn; intros.
-      cbv [cpscall cpsreturn]; rewrite body_cps_ok;
-        break_match; rewrite ?IHn; reflexivity.
+      revert f; revert R; revert s; induction n;
+        repeat match goal with
+               | _ => progress intros
+               | _ => progress cbv [cpsreturn cpscall] in *
+               | _ => progress cbn
+               | _ => progress rewrite ?body_cps_ok
+               | _ => progress rewrite ?IHn
+               | _ => progress break_match
+               | _ => reflexivity
+               end.
     Qed.
 
     Context (body_cps2 : A -> forall {R}, (A -> R) -> (B -> R) -> R).
     Fixpoint loop_cps2 (fuel : nat) (s : A) {R} (timeout:A->R) (ret:B->R) {struct fuel} : R :=
-      match fuel with
-      | O => timeout s
-      | S fuel' =>
-        body_cps2 s R
-                  (fun a => @loop_cps2 fuel' a R timeout ret)
-                  (fun b => ret b)
-      end.
+      body_cps2 s R
+                (fun a =>
+                   match fuel with
+                   | O => timeout a
+                   | S fuel' => @loop_cps2 fuel' a R timeout ret
+                   end)
+                (fun b => ret b).
 
     Context (body_cps2_ok : forall s {R} continue break,
                 body_cps2 s R continue break =
@@ -71,15 +84,22 @@ Module Import core.
       | inr b => ret b
       end.
     Proof.
-      revert ret; revert timeout; revert R; revert s;
-        induction n; intros; cbn; [reflexivity|].
-      rewrite body_cps2_ok.
-      destruct (body s); [|reflexivity].
-      rewrite IHn. reflexivity.
+      revert timeout; revert ret; revert R; revert s; induction n;
+        repeat match goal with
+               | _ => progress intros
+               | _ => progress cbv [cpsreturn cpscall] in *
+               | _ => progress cbn
+               | _ => progress rewrite ?body_cps2_ok
+               | _ => progress rewrite ?IHn
+               | _ => progress inversion_sum
+               | _ => progress subst
+               | _ => progress break_match
+               | _ => reflexivity
+               end.
     Qed.
 
-    Lemma loop_fuel_0 s : loop 0 s = inl s.
-    Proof. reflexivity. Qed.
+    Lemma loop_fuel_0 s : loop 0 s = body s.
+    Proof. cbv; break_match; reflexivity. Qed.
 
     Lemma loop_fuel_S_first n s : loop (S n) s =
                                   match body s with
@@ -102,7 +122,7 @@ Module Import core.
     Lemma loop_fuel_S_stable n s b (H : loop n s = inr b) : loop (S n) s = inr b.
     Proof.
       revert H; revert b; revert s; induction n; intros ? ? H.
-      { cbn [loop nat_rect] in H. congruence_sum. }
+      { cbn [loop nat_rect] in *; break_match_hyps; congruence_sum; congruence. }
       { rewrite loop_fuel_S_last.
         break_match; congruence_sum; reflexivity. }
     Qed.
@@ -128,8 +148,8 @@ Module Import core.
         { erewrite loop_fuel_S_stable by eassumption. congruence. } }
     Qed.
 
-    Lemma by_invariant' (inv P:_->Prop) measure f s0
-          (init : inv s0 /\ measure s0 < f)
+    Lemma by_invariant_fuel' (inv P:_->Prop) measure f s0
+          (init : inv s0 /\ measure s0 <= f)
           (step : forall s, inv s -> match body s with
                                      | inl s' => inv s' /\ measure s' < measure s
                                      | inr s' => P s'
@@ -140,24 +160,33 @@ Module Import core.
         end.
     Proof.
       revert dependent s0; induction f; intros; destruct_head'_and.
-      { exfalso; lia. }
+      { specialize (step s0 H); cbv; break_innermost_match; [lia|assumption]. }
       { rewrite loop_fuel_S_first.
         specialize (step s0 H); destruct (body s0); [|assumption].
         destruct step.
         exact (IHf a ltac:(split; (assumption || lia))). }
     Qed.
 
-    Lemma by_invariant (inv P:_->Prop) measure f s0
-          (init : inv s0 /\ measure s0 < f)
+    Lemma by_invariant_fuel (inv P:_->Prop) measure f s0
+          (init : inv s0 /\ measure s0 <= f)
           (step : forall s, inv s -> match body s with
                                      | inl s' => inv s' /\ measure s' < measure s
                                      | inr s' => P s'
                                      end)
       : exists b, loop f s0 = inr b /\ P b.
     Proof.
-      pose proof (by_invariant' inv P measure f s0);
+      pose proof (by_invariant_fuel' inv P measure f s0);
         specialize_by assumption; break_match_hyps; [contradiction|eauto].
     Qed.
+
+    Lemma by_invariant (inv P:_->Prop) measure s0
+          (init : inv s0)
+          (step : forall s, inv s -> match body s with
+                                     | inl s' => inv s' /\ measure s' < measure s
+                                     | inr s' => P s'
+                                     end)
+      : exists b, loop (measure s0) s0 = inr b /\ P b.
+    Proof. eapply by_invariant_fuel; eauto. Qed.
 
     (* Completeness proof *)
 
@@ -167,37 +196,36 @@ Module Import core.
                   match r with
                   | Some _ => r
                   | None =>
-                    match loop (S n) s with
+                    match loop n s with
                     | inl a => None
-                    | inr b => Some (S n)
+                    | inr b => Some n
                     end
                   end
                ) fuel.
 
     Lemma iterations_required_correct fuel s :
       (forall m, iterations_required fuel s = Some m ->
-                 1 <= m <= fuel /\
+                 m < fuel /\
                  exists b, forall n, (n < m -> exists a, loop n s = inl a) /\ (m <= n -> loop n s = inr b))
       /\
-      (iterations_required fuel s = None -> forall n, n <= fuel -> exists a, loop n s = inl a).
+      (iterations_required fuel s = None -> forall n, n < fuel -> exists a, loop n s = inl a).
     Proof.
       induction fuel; intros.
-      { cbn. split; intros; inversion_option.
-        replace n with 0 by lia. rewrite loop_fuel_0. eauto. }
+      { cbn. split; intros; inversion_option; lia. }
       { change (iterations_required (S fuel) s)
           with (match iterations_required fuel s with
-                | None => match loop (S fuel) s with
+                | None => match loop fuel s with
                           | inl _ => None
-                          | inr _ => Some (S fuel)
+                          | inr _ => Some fuel
                           end
                 | Some _ => iterations_required fuel s
                 end) in *.
         destruct (iterations_required fuel s) in *.
         { split; intros; inversion_option; subst.
           destruct (proj1 IHfuel _ eq_refl); split; [lia|assumption]. }
-        { destruct (loop (S fuel) s) eqn:HSf; split; intros; inversion_option; subst.
-          { intros. destruct (PeanoNat.Nat.eq_dec n (S fuel)); subst; eauto; [].
-            assert (n <= fuel) by lia. eapply IHfuel; congruence. }
+        { destruct (loop fuel s) eqn:HSf; split; intros; inversion_option; subst.
+          { intros. destruct (PeanoNat.Nat.eq_dec n fuel); subst; eauto; [].
+            assert (n < fuel) by lia. eapply IHfuel; congruence. }
           { split; [lia|].
             exists b; intros; split; intros.
             { eapply IHfuel; congruence || lia. }
@@ -206,14 +234,12 @@ Module Import core.
     Qed.
 
     Lemma iterations_required_step fuel s s' n
-          (Hs : iterations_required fuel s = Some n)
+          (Hs : iterations_required fuel s = Some (S n))
           (Hstep : body s = inl s')
-      : exists n', iterations_required fuel s' = Some n' /\ n = S n'.
+      : iterations_required fuel s' = Some n.
     Proof.
       eapply iterations_required_correct in Hs.
       destruct Hs as [Hn [b Hs]].
-      destruct n as [|n]; [pose proof (proj2 (Hs 0) ltac:(lia)) as Hx; inversion Hx|].
-      exists n; split; [|reflexivity].
       pose proof (proj2 (Hs (S n)) ltac:(lia)) as H.
       rewrite loop_fuel_S_first, Hstep in H.
       destruct (iterations_required fuel s') as [x|] eqn:Hs' in *; [f_equal|exfalso].
@@ -226,67 +252,60 @@ Module Import core.
           rewrite loop_fuel_S_first, Hstep in HX.
           pose proof (proj2 (Hs' x) ltac:(lia)).
           congruence. } }
-      { eapply iterations_required_correct in Hs'; [|exact (ltac:(lia) : n <= fuel)].
-        destruct Hs'.
-        congruence. }
+      { eapply iterations_required_correct in Hs'; destruct Hs' as [? Hs'];
+          [|exact Hn].
+        rewrite loop_fuel_S_last, H in Hs'; congruence. }
     Qed.
 
     Lemma invariant_complete (P:_->Prop) f s0 b (H:loop f s0 = inr b) (HP:P b)
       : exists inv measure,
-        (inv s0 /\ measure s0 < f)
+        (inv s0 /\ measure s0 <= f)
         /\ forall s, inv s -> match body s with
                               | inl s' => inv s' /\ measure s' < measure s
                               | inr s' => P s'
                               end.
     Proof.
-      set (measure f s :=
-             match iterations_required f s with
-             | None => 0
-             | Some s => pred s
-             end).
-      exists (fun s => match loop (S (measure f s)) s with
+      set (measure s := match iterations_required (S f) s with None => 0 | Some n => n end).
+      exists (fun s => match loop (measure s) s with
                        | inl a => False
                        | inr r => r = b end).
-      exists (measure f); split; [ |repeat match goal with |- _ /\ _ => split end..].
+      exists (measure); split; [ |repeat match goal with |- _ /\ _ => split end..].
       { cbv [measure].
-        destruct (iterations_required f s0) eqn:Hs0;
+        destruct (iterations_required (S f) s0) eqn:Hs0;
           eapply iterations_required_correct in Hs0;
-          [ .. | exact (ltac:(lia):f <= f)]; [|destruct_head'_ex; congruence].
-        destruct Hs0 as [? [? Hs0]].
-        replace (S (Nat.pred n)) with n by lia.
+          [ .. | exact (ltac:(lia):f <S f)]; [|destruct_head'_ex; congruence].
+        destruct Hs0 as [? [? Hs0]]; split; [|lia].
         pose proof (proj2 (Hs0 n) ltac:(lia)) as HH; rewrite HH.
-        split; [exact (loop_fuel_irrelevant _ _ _ _ _ HH H) | lia]. }
+        exact (loop_fuel_irrelevant _ _ _ _ _ HH H). }
       { intros s Hinv; destruct (body s) as [s'|c] eqn:Hstep.
-        { destruct (loop (S (measure f s)) s) eqn:Hs; [contradiction|subst].
+        { destruct (loop (measure s) s) eqn:Hs; [contradiction|subst].
           cbv [measure] in *.
-          destruct (iterations_required f s) eqn:Hs' in *;
-            [|rewrite loop_fuel_S_last in Hs; cbv in Hs; congruence].
-          destruct (iterations_required_step _ _ s' _ Hs' Hstep) as [? [HA ?]]; subst.
+          destruct (iterations_required (S f) s) eqn:Hs' in *; try destruct n;
+            try (rewrite loop_fuel_0 in Hs; congruence); [].
+          pose proof (iterations_required_step _ _ s' _ Hs' Hstep) as HA.
           rewrite HA.
           destruct (proj1 (iterations_required_correct _ _) _ HA) as [? [? [? HE']]].
           pose proof (HE' ltac:(constructor)) as HE; clear HE'.
           split; [|lia].
-          replace (S (Nat.pred (S x))) with (S x) in * by lia.
           rewrite loop_fuel_S_first, Hstep in Hs.
-          replace (S (Nat.pred x)) with x in * by lia; rewrite HE.
-          exact (loop_fuel_irrelevant _ _ _ _ _ HE Hs). }
-        { destruct (loop (S (measure f s)) s) eqn:Hs; [contradiction|subst].
+          break_match; congruence. }
+        { destruct (loop (measure s) s) eqn:Hs; [contradiction|].
           assert (HH: loop 1 s = inr c) by (cbn; rewrite Hstep; reflexivity).
-          rewrite (loop_fuel_irrelevant _ _ _ _ _ HH Hs); exact HP. } }
+          rewrite (loop_fuel_irrelevant _ _ _ _ _ HH Hs); congruence. } }
     Qed.
 
     Lemma invariant_iff f s0 P :
       (exists b, loop f s0 = inr b /\ P b)
       <->
       (exists inv measure,
-          (inv s0 /\ measure s0 < f)
+          (inv s0 /\ measure s0 <= f)
           /\ forall s, inv s -> match body s with
                                 | inl s' => inv s' /\ measure s' < measure s
                                 | inr s' => P s'
                                 end).
     Proof.
       repeat (intros || split || destruct_head'_ex || destruct_head'_and);
-        eauto using invariant_complete, by_invariant.
+        eauto using invariant_complete, by_invariant_fuel.
     Qed.
   End Loops.
 End core.
@@ -300,18 +319,27 @@ Module default.
       | inr s => s
       end.
 
-    Lemma by_invariant inv (P:_->Prop) measure f s0
-          (init : inv s0 /\ measure s0 < f)
+    Lemma by_invariant_fuel inv (P:_->Prop) measure f s0
+          (init : inv s0 /\ measure s0 <= f)
           (step: forall s, inv s -> match body s with
                                     | inl s' => inv s' /\ measure s' < measure s
                                     | inr s' => P s'
                                     end)
       : P (loop f s0).
     Proof.
-      edestruct (by_invariant body inv P measure f s0) as [x [HA HB]]; eauto; [].
+      edestruct (by_invariant_fuel body inv P measure f s0) as [x [HA HB]]; eauto; [].
       apply (f_equal (fun r : A + B => match r with inl s => default | inr s => s end)) in HA.
       cbv [loop]; break_match; congruence.
     Qed.
+
+    Lemma by_invariant (inv P:_->Prop) measure s0
+          (init : inv s0)
+          (step: forall s, inv s -> match body s with
+                                    | inl s' => inv s' /\ measure s' < measure s
+                                    | inr s' => P s'
+                                    end)
+      : P (loop (measure s0) s0).
+    Proof. eapply by_invariant_fuel; eauto. Qed.
   End Default.
 End default.
 
@@ -324,18 +352,27 @@ Module silent.
       | inr s => s
       end.
 
-    Lemma by_invariant inv (P:_->Prop) measure f s0
-          (init : inv s0 /\ measure s0 < f)
+    Lemma by_invariant_fuel inv (P:_->Prop) measure f s0
+          (init : inv s0 /\ measure s0 <= f)
           (step: forall s, inv s -> match body s with
                                     | inl s' => inv s' /\ measure s' < measure s
                                     | inr s' => P s'
                                     end)
       : P (loop f s0).
     Proof.
-      edestruct (by_invariant body inv P measure f s0) as [x [A B]]; eauto; [].
+      edestruct (by_invariant_fuel body inv P measure f s0) as [x [A B]]; eauto; [].
       apply (f_equal (fun r : state + state => match r with inl s => s | inr s => s end)) in A.
       cbv [loop]; break_match; congruence.
     Qed.
+
+    Lemma by_invariant (inv P:_->Prop) measure s0
+          (init : inv s0)
+          (step: forall s, inv s -> match body s with
+                                    | inl s' => inv s' /\ measure s' < measure s
+                                    | inr s' => P s'
+                                    end)
+      : P (loop (measure s0) s0).
+    Proof. eapply by_invariant_fuel; eauto. Qed.
   End Silent.
 End silent.
 
@@ -346,54 +383,75 @@ Module while.
             (body : state -> state).
 
     Fixpoint while f s :=
-      match f with
-      | O => s
-      | S f =>
-        if test s
-        then while f (body s)
-        else s
-      end.
+      if test s
+      then
+        let s := body s in
+        match f with
+        | O => s
+        | S f => while f s
+        end
+      else s.
 
     Local Definition lbody := fun s => if test s then inl (body s) else inr s.
 
     Lemma eq_loop f s : while f s = silent.loop lbody f s.
     Proof.
-      revert s; induction f; intros s; [reflexivity|].
-      cbn; cbv [silent.loop lbody] in *.
-      rewrite IHf.
-      cbn; cbv [silent.loop lbody].
-      break_match; reflexivity.
+      revert s; induction f; intros s;
+        repeat match goal with
+               | _ => progress cbn in *
+               | _ => progress cbv [silent.loop lbody] in *
+               | _ => rewrite IHf
+               | _ => progress break_match
+               | _ => congruence
+               end.
     Qed.
 
-    Lemma by_invariant inv P measure f s0
-          (init : inv s0 /\ measure s0 < f)
+    Lemma by_invariant_fuel inv P measure f s0
+          (init : inv s0 /\ measure s0 <= f)
           (step : forall s, inv s -> if test s
                                      then inv (body s) /\ measure (body s) < measure s
                                      else P s)
       : P (while f s0).
     Proof.
       rewrite eq_loop.
-      eapply silent.by_invariant; eauto; []; intros s H; cbv [lbody].
+      eapply silent.by_invariant_fuel; eauto; []; intros s H; cbv [lbody].
       specialize (step s H); destruct (test s); eauto.
     Qed.
+
+    Lemma by_invariant (inv P:_->Prop) measure s0
+          (init : inv s0)
+          (step : forall s, inv s -> if test s
+                                     then inv (body s) /\ measure (body s) < measure s
+                                     else P s)
+      : P (while (measure s0) s0).
+    Proof. eapply by_invariant_fuel; eauto. Qed.
     
     Context (body_cps : state ~> state).
 
     Fixpoint while_cps f s :~> state :=
-      match f with
-      | O => return s
-      | S f =>
-        if test s
-        then s <- body_cps s; while_cps f s
-        else return s
-      end.
+      if test s
+      then
+        s <- body_cps s; 
+          match f with
+          | O => return s
+                      | S f =>while_cps f s
+          end
+      else return s.
 
     Context (body_cps_ok : forall s {R} f, body_cps s R f = f (body s)).
     Lemma loop_cps_ok n s {R} f : while_cps n s R f = f (while n s).
     Proof.
-      revert s; induction n; intros s; [reflexivity|].
-      cbn; break_match;
-        cbv [cpscall cpsreturn]; rewrite ?body_cps_ok, ?IHn; reflexivity.
+      revert s; induction n; intros s; 
+        repeat match goal with
+               | _ => progress intros
+               | _ => progress cbv [cpsreturn cpscall] in *
+               | _ => progress cbn
+               | _ => progress rewrite ?body_cps_ok
+               | _ => progress rewrite ?IHn
+               | _ => progress inversion_sum
+               | _ => progress break_match
+               | _ => reflexivity
+               end.
     Qed.
   End While.
 End while.
